src/Std/Data/Iterators/Consumers/Monadic/Loop.lean
@@ -62,8 +62,9 @@ class IteratorLoop (α : Type w) (m : Type w → Type w') {β : Type w} [Iterato
   forIn : ∀ (_lift : (γ : Type w) → m γ → n γ) (γ : Type w),
       (plausible_forInStep : β → γ → ForInStep γ → Prop) →
       IteratorLoop.WellFounded α m plausible_forInStep →
-      IterM (α := α) m β → γ →
-      ((b : β) → (c : γ) → n (Subtype (plausible_forInStep b c))) → n γ
+      (it : IterM (α := α) m β) → γ →
+      ((b : β) → it.IsPlausibleIndirectOutput b → (c : γ) → n (Subtype (plausible_forInStep b c))) →
+      n γ
 
 /--
 `IteratorLoopPartial α m` provides efficient implementations of loop-based consumers for `α`-based
@@ -76,7 +77,8 @@ provided by the standard library.
 class IteratorLoopPartial (α : Type w) (m : Type w → Type w') {β : Type w} [Iterator α m β]
     (n : Type w → Type w'') where
   forInPartial : ∀ (_lift : (γ : Type w) → m γ → n γ) {γ : Type w},
-      IterM (α := α) m β → γ → ((b : β) → (c : γ) → n (ForInStep γ)) → n γ
+      (it : IterM (α := α) m β) → γ →
+      ((b : β) → it.IsPlausibleIndirectOutput b → (c : γ) → n (ForInStep γ)) → n γ
 
 class IteratorSize (α : Type w) (m : Type w → Type w') {β : Type w} [Iterator α m β] where
   size : IterM (α := α) m β → m (ULift Nat)
@@ -115,16 +117,20 @@ def IterM.DefaultConsumers.forIn {m : Type w → Type w'} {α : Type w} {β : Ty
     (plausible_forInStep : β → γ → ForInStep γ → Prop)
     (wf : IteratorLoop.WellFounded α m plausible_forInStep)
     (it : IterM (α := α) m β) (init : γ)
-    (f : (b : β) → (c : γ) → n (Subtype (plausible_forInStep b c))) : n γ :=
+    (f : (b : β) → it.IsPlausibleIndirectOutput b → (c : γ) → n (Subtype (plausible_forInStep b c))) : n γ :=
   haveI : WellFounded _ := wf
   letI : MonadLift m n := ⟨fun {γ} => lift γ⟩
   do
     match ← it.step with
-    | .yield it' out _ =>
-      match ← f out init with
-      | ⟨.yield c, _⟩ => IterM.DefaultConsumers.forIn lift _ plausible_forInStep wf it' c f
+    | .yield it' out h =>
+      match ← f out (.direct ⟨_, h⟩) init with
+      | ⟨.yield c, _⟩ =>
+        IterM.DefaultConsumers.forIn lift _ plausible_forInStep wf it' c
+          (fun out h' acc => f out (.indirect ⟨_, rfl, h⟩ h') acc)
       | ⟨.done c, _⟩ => return c
-    | .skip it' _ => IterM.DefaultConsumers.forIn lift _ plausible_forInStep wf it' init f
+    | .skip it' h =>
+      IterM.DefaultConsumers.forIn lift _ plausible_forInStep wf it' init
+        (fun out h' acc => f out (.indirect ⟨_, rfl, h⟩ h') acc)
     | .done _ => return init
 termination_by IteratorLoop.WFRel.mk wf it init
 decreasing_by
@@ -159,15 +165,19 @@ partial def IterM.DefaultConsumers.forInPartial {m : Type w → Type w'} {α : T
     {n : Type w → Type w''} [Monad n]
     (lift : ∀ γ, m γ → n γ) (γ : Type w)
     (it : IterM (α := α) m β) (init : γ)
-    (f : (b : β) → (c : γ) → n (ForInStep γ)) : n γ :=
+    (f : (b : β) → it.IsPlausibleIndirectOutput b → (c : γ) → n (ForInStep γ)) : n γ :=
   letI : MonadLift m n := ⟨fun {γ} => lift γ⟩
   do
     match ← it.step with
-    | .yield it' out _ =>
-      match ← f out init with
-      | .yield c => IterM.DefaultConsumers.forInPartial lift _ it' c f
+    | .yield it' out h =>
+      match ← f out (.direct ⟨_, h⟩) init with
+      | .yield c =>
+        IterM.DefaultConsumers.forInPartial lift _ it' c
+          fun out h' acc => f out (.indirect ⟨_, rfl, h⟩ h') acc
       | .done c => return c
-    | .skip it' _ => IterM.DefaultConsumers.forInPartial lift _ it' init f
+    | .skip it' h =>
+      IterM.DefaultConsumers.forInPartial lift _ it' init
+        fun out h' acc => f out (.indirect ⟨_, rfl, h⟩ h') acc
     | .done _ => return init
 
 /--
@@ -202,27 +212,28 @@ theorem IteratorLoop.wellFounded_of_finite {m : Type w → Type w'}
     exact WellFoundedRelation.wf
 
 /--
-This `ForIn`-style loop construct traverses a finite iterator using an `IteratorLoop` instance.
+This `ForIn'`-style loop construct traverses a finite iterator using an `IteratorLoop` instance.
 -/
 @[always_inline, inline]
-def IteratorLoop.finiteForIn {m : Type w → Type w'} {n : Type w → Type w''}
+def IteratorLoop.finiteForIn' {m : Type w → Type w'} {n : Type w → Type w''}
     {α : Type w} {β : Type w} [Iterator α m β] [Finite α m] [IteratorLoop α m n]
     (lift : ∀ γ, m γ → n γ) :
-    ForIn n (IterM (α := α) m β) β where
-  forIn {γ} [Monad n] it init f :=
+    ForIn' n (IterM (α := α) m β) β ⟨fun it out => it.IsPlausibleIndirectOutput out⟩ where
+  forIn' {γ} [Monad n] it init f :=
     IteratorLoop.forIn (α := α) (m := m) lift γ (fun _ _ _ => True)
       wellFounded_of_finite
-      it init ((⟨·, .intro⟩) <$> f · ·)
+      it init (fun out h acc => (⟨·, .intro⟩) <$> f out h acc)
 
 instance {m : Type w → Type w'} {n : Type w → Type w''}
     {α : Type w} {β : Type w} [Iterator α m β] [Finite α m] [IteratorLoop α m n]
     [MonadLiftT m n] :
-    ForIn n (IterM (α := α) m β) β := IteratorLoop.finiteForIn (fun _ => monadLift)
+    ForIn' n (IterM (α := α) m β) β ⟨fun it out => it.IsPlausibleIndirectOutput out⟩ :=
+  IteratorLoop.finiteForIn' (fun _ => monadLift)
 
 instance {m : Type w → Type w'} {n : Type w → Type w''}
     {α : Type w} {β : Type w} [Iterator α m β] [IteratorLoopPartial α m n] [MonadLiftT m n] :
-    ForIn n (IterM.Partial (α := α) m β) β where
-  forIn it init f :=
+    ForIn' n (IterM.Partial (α := α) m β) β ⟨fun it out => it.it.IsPlausibleIndirectOutput out⟩ where
+  forIn' it init f :=
     IteratorLoopPartial.forInPartial (α := α) (m := m) (fun _ => monadLift) it.it init f
 
 instance {m : Type w → Type w'} {n : Type w → Type w''}
