src/Std/Data/Iterators/Consumers/Loop.lean
@@ -24,9 +24,11 @@ namespace Std.Iterators
 
 instance (α : Type w) (β : Type w) (n : Type w → Type w') [Monad n]
     [Iterator α Id β] [Finite α Id] [IteratorLoop α Id n] :
-    ForIn n (Iter (α := α) β) β where
-  forIn it init f :=
-    IteratorLoop.finiteForIn (fun δ (c : Id δ) => pure c.run) |>.forIn it.toIterM init f
+    ForIn' n (Iter (α := α) β) β ⟨fun it out => it.IsPlausibleIndirectOutput out⟩ where
+  forIn' it init f :=
+    IteratorLoop.finiteForIn' (fun δ (c : Id δ) => pure c.run) |>.forIn' it.toIterM init
+        fun out h acc =>
+          f out (Iter.isPlausibleIndirectOutput_iff_isPlausibleIndirectOutput_toIterM.mpr h) acc
 
 instance (α : Type w) (β : Type w) (n : Type w → Type w') [Monad n]
     [Iterator α Id β] [IteratorLoopPartial α Id n] :
