src/Std/Data/Ranges/Nat.lean
@@ -9,6 +9,22 @@ open Std.Iterators
 instance : Succ? Nat where
   succ? n := some (n + 1)
 
+instance : LawfulLESucc? Nat where
+  le_rfl := Nat.le_refl _
+  le_succ?_of_le hle h := by
+    simp only [Succ?.succ?, Option.some.injEq] at h
+    omega
+  le_succAtIdx?_of_le {a b c n} hle h := by
+    simp only [Succ?.succAtIdx?, Option.bind_eq_bind] at h
+    induction n generalizing b c with
+    | zero => simp_all [Nat.repeat]
+    | succ n ih =>
+      simp only [Nat.repeat, Option.bind_eq_some_iff] at h ih
+      rcases h with ⟨c', hc', h⟩
+      cases h
+      specialize ih hle hc'
+      omega
+
 instance (stepSize : Nat) (h) :
     Finite (Range.SuccIterator (α := Nat) stepSize (· ≤ n) h) Id := by
   unfold Range.SuccIterator
